added the auth part to pingpong

raft/src/example/SimpleExample.v
@@ -12,23 +12,27 @@ Require Export Process.
 
 Section PingPong.
 
+  (*+ declare the basics +*)
+  (*! node definition !*)
   (* Define the type of nodes that are used within the protocol *)
   Inductive PPnode :=
   | PPn. (* don't distinguish between nodes or is some client (initially node) needed? *)
 
-  (* Define the type of messages which can be send between nodes and internally  *)
-  Inductive PPmsg :=
-  | PPping (* Either send a Ping if this is the first round or reply to a pong *)
-  | PPong. (* Reply to some incoming ping message *)
 
   (* Show that the node definition holds for the decidable equality (Deq) *)
   Lemma Deq_PPnode : Deq PPnode.
   Proof.
     introv. destruct x, y. prove_dec.
-    Qed.
+  Qed.
 
   (* Instantiate the abstract type node with the protocol node definition *)
   Instance PP_I_Node: Node := MkNode PPnode Deq_PPnode.
+
+  (*! message definition !*)
+  (* Define the type of messages which can be send between nodes and internally  *)
+  Inductive PPmsg :=
+  | PPping (* Either send a Ping if this is the first round or reply to a pong *)
+  | PPong. (* Reply to some incoming ping message *)
 
   (* Instantiate the abstract message type with the protocol message definition *)
   Instance PP_I_Msg : Msg := MkMsg PPmsg.
@@ -43,14 +47,85 @@ Section PingPong.
   (* Instantiate the abstract message status with the function describing it *)
   Instance PP_I_MsgStatus : MsgStatus := MkMsgStatus PP_msg_status.
 
-  (* Declare the internal states for the nodes.
+  (*! state definition !*)
+  (* Declare the states for the nodes.
    * Different node types may have different states. *)
   Inductive PPstate := PPst.
 
   (* Define the state update function as simple echo. *)
   Definition echo : MSUpdate PPstate :=
     (* Given some msg and the current state, the next state is the same but
-     * the input message is directed back to all other nodes in the network. *)
+     * the input message is directed back to all other nodes in the network
+     * via directed messages. *)
     fun state input => (state, [MkDMsg input [PPn] 0]).
+
+  (* declare the internal state machine ?? *)
+  Arguments MkSM      [S] [I] [O] _ _ _.
+  Arguments sm_halted [S] [I] [O] _.
+  Arguments sm_state  [S] [I] [O] _.
+  Arguments sm_update [S] [I] [O] _ _ _.
+
+  (* define the internal state machine for a ping pong node *)
+  Definition PPnodeSM : MStateMachine PPstate :=
+    mkSSM echo PPst.
+
+  (* match node types with their states *)
+  Definition PPState (n : name) :=
+    match n with
+    | PPn => PPstate
+    end.
+
+  (* match the state machine for the node type and return the next state *)
+  Definition PPusys : MUSystem PPState :=
+    fun name =>
+      match name return StateMachine (PPState name) msg DirectedMsgs with
+      | PPn => PPnodeSM
+      end.
+
+  (* build the real process with some initial state machine *)
+  Definition PPsys  : System :=
+    fun name =>
+      match name with
+      | PPn => build_sprocess echo PPst
+      end.
+
+  (*+ declare the authentication +*)
+  (* create new key *)
+  Instance PP_I_Key : Key := MkKey unit unit.
+
+  (* define what type is data *)
+  Instance PP_I_Data : Data := MkData PPmsg.
+
+  (* create a new authentication token *)
+  Instance PP_I_AuthTok : AuthTok := MkAuthTok unit Deq_unit.
+
+  Instance PP_I_AuthFun : AuthFun :=
+    MkAuthFun
+      (fun _ _ => [tt])
+      (fun _ _ _ _ => true).
+
+  Definition PPdata_auth : name -> PPmsg -> option name :=
+    fun n m =>
+      match m with
+      | PPping => Some PPn
+      | PPong  => Some PPn
+      end.
+
+  (* Instantiate the abstract DataAuth type with the protocol implementation *)
+  Instance PP_I_DataAuth : DataAuth := MkDataAuth PPdata_auth.
+
+  (* Instantiate the ContainedAuthData which creates mesages with
+   * multiple authenticated data? *)
+  Instance PP_I_ContainedAuthData : ContainedAuthData :=
+    MkContainedAuthData
+      (fun m => [MkAuthData m [tt]]).
+
+  (* add some hints to the proofer *)
+  Hint Rewrite @map_option_option_map : option.
+  Hint Rewrite @option_map_option_map : option.
+  Hint Resolve if_not_first_if_first : eo.
+
+  (*+ proofs about the event ordering +*)
+  (* currently left out*)
 
 End PingPong.
